src/semantics.lean
@@ -25,17 +25,17 @@ instance (M : model L) : inhabited M.dom := ⟨M.one⟩
 
 @[simp] def term.val (e : ℕ → |M|) (t : term L) : M.dom := (t.val e).head
 
-@[simp] def form.val : (ℕ → |M|) → form L → Prop
-| _ (form.const c) := M.pr c dvector.nil
-| e (form.app p v) := M.pr p (v.val e)
+@[simp] def formula.val : (ℕ → |M|) → formula L → Prop
+| _ (formula.const c) := M.pr c dvector.nil
+| e (formula.app p v) := M.pr p (v.val e)
 | e (t =̇ u)        := t.val e = u.val e
 | e (p →̇ q)       := p.val e → q.val e
 | e (¬̇p)           := ¬(p.val e)
 | e (Ȧp)           := ∀ d : M.dom, (p.val (d ^ˢ e))
 
-notation M` ⊧[`:80 e`] `p :50 := @form.val _ M e p
+notation M` ⊧[`:80 e`] `p :50 := @formula.val _ M e p
 
-def models (M : model L) (p : form L) : Prop := ∀ (e : ℕ → |M|), M ⊧[e] p
+def models (M : model L) (p : formula L) : Prop := ∀ (e : ℕ → |M|), M ⊧[e] p
 infix ` ⊧ `:50 := models
 
 def modelsth (M : model L) (T : theory L) : Prop := ∀ p, p ∈ T → M ⊧ p
@@ -51,43 +51,43 @@ lemma rew_val_eq : ∀ (s : ℕ → term L) {n} (t : vecterm L n) (e : ℕ → |
 @[simp] lemma sf_slide_val {n} (t : vecterm L n) : ∀ (e : ℕ → |M|) d, t.sf.val (d ^ˢ e) = t.val e :=
 by induction t; simp[slide]; simp*
 
-lemma rew_val_iff : ∀ (s : ℕ → term L) (p : form L) (e : ℕ → |M|),
+lemma rew_val_iff : ∀ (s : ℕ → term L) (p : formula L) (e : ℕ → |M|),
   (p.rew s).val e ↔ p.val (λ n, (s n).val e)
-| _ (form.const c) _ := by simp[form.rew]
-| _ (form.app p v) _ := by simp[form.rew, rew_val_eq]
-| _ (t =̇ u)        _ := by simp[form.rew, term.val, rew_val_eq]
-| _ (p →̇ q)       _ := by simp[form.rew, rew_val_iff _ p, rew_val_iff _ q]
-| _ (¬̇p)           _ := by simp[form.rew, rew_val_iff _ p]
-| s (Ȧp)           e := by { simp[form.rew, rew_val_iff _ p], refine forall_congr (λ d, _),
+| _ (formula.const c) _ := by simp[formula.rew]
+| _ (formula.app p v) _ := by simp[formula.rew, rew_val_eq]
+| _ (t =̇ u)        _ := by simp[formula.rew, term.val, rew_val_eq]
+| _ (p →̇ q)       _ := by simp[formula.rew, rew_val_iff _ p, rew_val_iff _ q]
+| _ (¬̇p)           _ := by simp[formula.rew, rew_val_iff _ p]
+| s (Ȧp)           e := by { simp[formula.rew, rew_val_iff _ p], refine forall_congr (λ d, _),
     have : (λ n, (((#0 ^ˢ λ x, (s x).sf) n).val (d ^ˢ e)).head) = (d ^ˢ λ n, ((s n).val e)),
     { funext n,cases n; simp[slide, term.val, vecterm.val] },
     simp[this] }
 
-@[simp] lemma sf_slide_val_iff : ∀ (p : form L) (e : ℕ → |M|) d, p.sf.val (d ^ˢ e) = p.val e
-| (form.const c) _ _ := rfl
-| (form.app p v) _ _ := by simp
+@[simp] lemma sf_slide_val_iff : ∀ (p : formula L) (e : ℕ → |M|) d, p.sf.val (d ^ˢ e) = p.val e
+| (formula.const c) _ _ := rfl
+| (formula.app p v) _ _ := by simp
 | (t =̇ u)        _ _ := by simp[term.val]
 | (p →̇ q)       _ _ := by simp[sf_slide_val_iff p, sf_slide_val_iff q]
 | (¬̇p)           _ _ := by simp[sf_slide_val_iff p]
-| (Ȧp)           _ _ := by simp[term.val, form.sf, rew_val_iff, slide]
+| (Ȧp)           _ _ := by simp[term.val, formula.sf, rew_val_iff, slide]
 
 private lemma modelsth_sf {T} : M ⊧ₜₕ T → M ⊧ₜₕ ⇑T := λ h p hyp_p e,
 by { cases hyp_p with p hyp_p', simp[rew_val_iff],
      refine h _ hyp_p' _ }
 
 @[simp] lemma models_ex {p} {e : ℕ → |M|} : (Ėp).val e ↔ ∃ d, p.val (d ^ˢ e) :=
-by simp[form.ex, models, form.subst₁, rew_val_iff]
+by simp[formula.ex, models, formula.subst₁, rew_val_iff]
 
 @[simp] lemma models_and {p q} {e : ℕ → |M|} : (p ⩑ q).val e ↔ (p.val e ∧ q.val e) :=
-by simp[form.and]
+by simp[formula.and]
 
 @[simp] lemma models_iff {p q} {e : ℕ → |M|} : (p ↔̇ q).val e ↔ (p.val e ↔ q.val e) :=
-by simp[form.iff]; exact iff_def.symm
+by simp[formula.iff]; exact iff_def.symm
 
 @[simp] lemma models_equals : ∀ {n} (v₁ v₂ : vecterm L n) (e : ℕ → |M|),
   (v₁ ≡̇ v₂).val e ↔ v₁.val e = v₂.val e
-| 0     t₁ t₂ e := by simp[form.val]
-| (n+1) (vecterm.cons t₁ v₁) (vecterm.cons t₂ v₂) e := by simp[form.val, models_equals v₁ v₂]
+| 0     t₁ t₂ e := by simp[formula.val]
+| (n+1) (vecterm.cons t₁ v₁) (vecterm.cons t₂ v₂) e := by simp[formula.val, models_equals v₁ v₂]
 
 theorem soundness {T : theory L} : ∀ {p}, T ⊢̇ p → ∀ {M}, M ⊧ₜₕ T → M ⊧ p := λ p hyp,
 begin
@@ -103,9 +103,9 @@ begin
   case fopl.provable.p2 : T p q r
   { intros M hyp_T e h₁ h₂ h₃, exact (h₁ h₃) (h₂ h₃) },
   case fopl.provable.p3 : T p q
-  { intros M hyp_T e h₁, simp[form.val], contrapose, exact h₁ },
+  { intros M hyp_T e h₁, simp[formula.val], contrapose, exact h₁ },
   case fopl.provable.q1 : T p t
-  { intros M hyp_T e h, simp[form.subst₁, rew_val_iff] at h ⊢,
+  { intros M hyp_T e h, simp[formula.subst₁, rew_val_iff] at h ⊢,
     have : (λ n, (vecterm.val e (t ^ˢ vecterm.var $ n)).head) = (t.val e) ^ˢ e,
     { funext n, cases n; simp[slide, term.val, vecterm.val] },
     rw this, exact h _ },
@@ -114,15 +114,15 @@ begin
   case fopl.provable.q3 : T p
   { intros M hyp_T e h d, simp, exact h },
   case fopl.provable.e1 : T t
-  { intros M hyp_T e, simp[form.val] },
+  { intros M hyp_T e, simp[formula.val] },
   case fopl.provable.e2 : T t₁ t₂
-  { intros M hyp_T e, simp[form.val], refine eq.symm },
+  { intros M hyp_T e, simp[formula.val], refine eq.symm },
   case fopl.provable.e3 : T t₁ t₂ t₃
-  { intros M hyp_T e, simp[form.val], refine eq.trans },
+  { intros M hyp_T e, simp[formula.val], refine eq.trans },
   case fopl.provable.e4 : T n t₁ t₂ f
-  { intros M hyp_T e, simp[form.val], refine λ eqn, (by simp[eqn]) },
+  { intros M hyp_T e, simp[formula.val], refine λ eqn, (by simp[eqn]) },
   case fopl.provable.e5 : T n t₁ t₂ f
-  { intros M hyp_T e, simp[form.val], refine λ eqn, (by simp[eqn]) },
+  { intros M hyp_T e, simp[formula.val], refine λ eqn, (by simp[eqn]) },
 end
 
 theorem model_consistent {T : theory L} : M ⊧ₜₕ T → theory.consistent T :=
@@ -138,28 +138,28 @@ lemma eval_eq : ∀ {n} {v : vecterm L n} {e₁ e₂ : ℕ → |M|},
 | _     (vecterm.app f v)  e₁ e₂ a := by { simp[vecterm.arity] at *, 
     simp[eval_eq a] } 
 
-lemma eval_iff : ∀ {p : form L} {e₁ e₂ : ℕ → |M|},
+lemma eval_iff : ∀ {p : formula L} {e₁ e₂ : ℕ → |M|},
   (∀ n, n < p.arity → e₁ n = e₂ n) → (M ⊧[e₁] p ↔ M ⊧[e₂] p)
-| (form.const _) _  _  _ := by simp* at *
-| (form.app p v) e₁ e₂ a := by { simp[sentence, form.arity] at*, simp[eval_eq a] }
-| (t =̇ u)        e₁ e₂ a := by { simp[sentence, form.arity] at*,
+| (formula.const _) _  _  _ := by simp* at *
+| (formula.app p v) e₁ e₂ a := by { simp[sentence, formula.arity] at*, simp[eval_eq a] }
+| (t =̇ u)        e₁ e₂ a := by { simp[sentence, formula.arity] at*,
   simp[eval_eq (λ n h, a _ (or.inl h)), eval_eq (λ n h, a _ (or.inr h))] }
-| (p →̇ q)       e₁ e₂ a := by { simp[sentence, form.arity] at*,
+| (p →̇ q)       e₁ e₂ a := by { simp[sentence, formula.arity] at*,
     simp[eval_iff (λ n h, a _ (or.inl h)), eval_iff (λ n h, a _ (or.inr h))] }
-| (¬̇p)           e₁ e₂ a := by { simp[sentence, form.arity] at*,
+| (¬̇p)           e₁ e₂ a := by { simp[sentence, formula.arity] at*,
     simp[eval_iff a] }
-| (Ȧp)           e₁ e₂ a := by { simp[sentence, form.arity] at*,
+| (Ȧp)           e₁ e₂ a := by { simp[sentence, formula.arity] at*,
     have : ∀ (d : |M|), p.val (d ^ˢ e₁) ↔ p.val (d ^ˢ e₂),
     { intros d, refine eval_iff (λ n eqn, _),
       cases n, { simp }, simp, refine a _ (nat.lt_sub_right_of_add_lt eqn) },
     exact forall_congr this }
 
-lemma eval_sentence_iff {p : form L} {e : ℕ → |M|} (a : sentence p) : M ⊧[e] p ↔ M ⊧ p :=
+lemma eval_sentence_iff {p : formula L} {e : ℕ → |M|} (a : sentence p) : M ⊧[e] p ↔ M ⊧ p :=
 ⟨λ h e, by { refine (eval_iff $ λ n h, _).1 h, exfalso,
  simp[sentence] at*, rw[a] at h, exact nat.not_lt_zero n h},
  λ h, h e⟩
 
-lemma nfal_models_iff : ∀ {n} {p : form L}, M ⊧ p ↔ M ⊧ nfal p n
+lemma nfal_models_iff : ∀ {n} {p : formula L}, M ⊧ p ↔ M ⊧ nfal p n
 | 0     _ := iff.rfl
 | (n+1) p := by { simp[@nfal_models_iff n p], refine ⟨λ h e d, h _, λ h e, _⟩,
   have : (e 0) ^ˢ (λ x, e (x + 1)) = e, { ext x, cases x; simp },
